Verbatim/state.v
@@ -40,7 +40,12 @@ Module Type STATE (Import R : regex.T).
       accepting (transition_list bs (init_state e)) = accepting (init_state (derivative_list bs e)).
   
   Parameter accepts_matches : forall(s : String) (e : regex),
-    true = accepts s (init_state e) <-> exp_match s e.
+      true = accepts s (init_state e) <-> exp_match s e.
+
+  Parameter stt_compare : State -> State -> comparison.
+  Parameter stt_compare_eq : forall x y, stt_compare x y = Eq <-> x = y.
+  Parameter stt_compare_trans : forall c x y z,
+      stt_compare x y = c -> stt_compare y z = c -> stt_compare x z = c.
 
 End STATE.
 
@@ -49,28 +54,6 @@ Module DefsFn (R : regex.T) (Ty : STATE R).
   Import Ty.
   Import R.Defs.
   Import R.Ty.
-
-  
-  Module Export comparable.
-
-    Definition stt_compare (s1 s2 : State) : comparison :=
-      re_compare (init_state_inv s1) (init_state_inv s2).
-
-    Lemma stt_compare_eq : forall x y,
-        stt_compare x y = Eq <-> x = y.
-    Proof.
-      intros.
-    Admitted.
-
-    Lemma stt_compare_trans : forall c x y z,
-        stt_compare x y = c -> stt_compare y z = c -> stt_compare x z = c.
-    Admitted.
-
-    (*
-    Lemma stt_eq_dec : forall (x y : State), {x = y} + {x <> y}.
-    Admitted.*)
-
-  End comparable.
     
 
   Module State_as_UCT <: UsualComparableType.
